ulib: adding some interfaces

ulib/FStar.GSet.fst
@@ -51,3 +51,15 @@ let mem_of_set     #a f x     = ()
 let lemma_equal_intro #a s1 s2 = ()
 let lemma_equal_elim  #a s1 s2 = ()
 let lemma_equal_refl  #a s1 s2 = ()
+
+let disjoint_not_in_both (a:Type) (s1:set a) (s2:set a) :
+  Lemma
+    (requires (disjoint s1 s2))
+    (ensures (forall (x:a).{:pattern (mem x s1) \/ (mem x s2)} mem x s1 ==> ~(mem x s2)))
+  [SMTPat (disjoint s1 s2)]
+= let f (x:a) : Lemma (~(mem x (intersect s1 s2))) = () in
+  FStar.Classical.forall_intro f
+let lemma_disjoint_subset (#a:Type) (s1:set a) (s2:set a) (s3:set a)
+  : Lemma (requires (disjoint s1 s2 /\ subset s3 s1))
+          (ensures  (disjoint s3 s2))
+  = ()
